WIP remove permanent state from world

theories/model/region_invariants_definitions.v
@@ -6,73 +6,20 @@ Section region_invariants_definitions.
   (* We will first define the standard STS for the shared part of the heap *)
   Inductive region_type :=
   | Temporary
-  | Permanent
   | Revoked.
 
   Global Instance LeibnizEquiv_region_type : @LeibnizEquiv region_type (@eq region_type).
   Proof. rewrite /LeibnizEquiv; intros ? ? ?; done. Defined.
 
   Inductive std_rel_pub : region_type -> region_type -> Prop :=
-  | Std_pub_Revoked_Temporary : std_rel_pub Revoked Temporary
-  | Std_pub_Revoked_Permanent : std_rel_pub Revoked Permanent.
+  | Std_pub_Revoked_Temporary : std_rel_pub Revoked Temporary.
 
   Inductive std_rel_priv : region_type -> region_type -> Prop :=
-  | Std_priv_Temporary_Revoked : std_rel_priv Temporary Revoked
-  | Std_priv_Temporary_Permanent : std_rel_priv Temporary Permanent.
+  | Std_priv_Temporary_Revoked : std_rel_priv Temporary Revoked.
 
   (* --------------------------------------------------------------------------------- *)
   (* ------------------------- LEMMAS ABOUT STD TRANSITIONS -------------------------- *)
   (* --------------------------------------------------------------------------------- *)
-
-  Lemma std_rel_pub_Permanent (ρ : region_type) :
-    std_rel_pub Permanent ρ → ρ = Permanent.
-  Proof.
-    intros Hrel.
-    inversion Hrel.
-  Qed.
-
-  Lemma std_rel_pub_rtc_Permanent (ρ1 ρ2 : region_type) :
-    ρ1 = Permanent →
-    rtc std_rel_pub ρ1 ρ2 → ρ2 = Permanent.
-  Proof.
-    intros Hρ1 Hrtc.
-    induction Hrtc;auto.
-    subst. apply IHHrtc. apply std_rel_pub_Permanent; auto.
-  Qed.
-
-  Lemma std_rel_priv_Permanent (ρ : region_type) :
-    std_rel_priv Permanent ρ → ρ = Permanent.
-  Proof.
-    intros Hrel.
-    inversion Hrel; done.
-  Qed.
-
-  Lemma std_rel_priv_rtc_Permanent (ρ1 ρ2 : region_type) :
-    ρ1 = Permanent →
-    rtc std_rel_priv ρ1 ρ2 → ρ2 = Permanent.
-  Proof.
-    intros Hρ1 Hrtc.
-    induction Hrtc;auto.
-    subst. apply IHHrtc. apply std_rel_priv_Permanent; auto.
-  Qed.
-
-  Lemma std_rel_Permanent (ρ : region_type) :
-    (std_rel_pub Permanent ρ ∨ std_rel_priv Permanent ρ) → ρ = Permanent.
-  Proof.
-    intros Hrel.
-    destruct Hrel.
-    + by apply std_rel_pub_Permanent.
-    + by apply std_rel_priv_Permanent.
-  Qed.
-
-  Lemma std_rtc_Permanent (ρ1 ρ2 : region_type) :
-    ρ1 = Permanent →
-    rtc (λ x y : region_type, std_rel_pub x y ∨ std_rel_priv x y) ρ1 ρ2 → ρ2 = Permanent.
-  Proof.
-    intros Hρ1 Hrtc.
-    induction Hrtc;auto.
-    subst. apply IHHrtc. apply std_rel_Permanent; auto.
-  Qed.
 
   Lemma std_rel_priv_Revoked (ρ : region_type) :
     std_rel_priv Revoked ρ → ρ = Revoked.
@@ -88,18 +35,6 @@ Section region_invariants_definitions.
     intros Hρ1 Hrtc.
     induction Hrtc;auto.
     subst. apply IHHrtc. apply std_rel_priv_Revoked; auto.
-  Qed.
-
-  Lemma std_rel_rtc_Permanent (ρ1 ρ2 : region_type) :
-    ρ1 = Permanent →
-    rtc (λ ρ0 ρ0' : region_type, std_rel_pub ρ0 ρ0' ∨ std_rel_priv ρ0 ρ0') ρ1 ρ2 →
-    ρ2 = Permanent.
-  Proof.
-    intros Hρ1 Hrtc.
-    induction Hrtc as [|ρ0 ρ1 ρ2 Hrel];auto.
-    subst. destruct Hrel as [Hrel | Hrel].
-    - apply std_rel_pub_Permanent in Hrel; auto.
-    - apply std_rel_priv_Permanent in Hrel; auto.
   Qed.
 
   Lemma std_rel_pub_Temporary (ρ : region_type) :
@@ -119,7 +54,7 @@ Section region_invariants_definitions.
   Qed.
 
   Lemma std_rel_pub_Revoked (ρ : region_type) :
-    std_rel_pub Revoked ρ → ρ = Permanent ∨ ρ = Temporary.
+    std_rel_pub Revoked ρ → ρ = Temporary.
   Proof.
     intros Hrel.
     inversion Hrel; auto.
@@ -127,13 +62,12 @@ Section region_invariants_definitions.
 
   Lemma std_rel_pub_rtc_Revoked (ρ1 ρ2 : region_type) :
     ρ1 = Revoked →
-    rtc std_rel_pub ρ1 ρ2 → ρ2 = Permanent ∨ ρ2 = Temporary ∨ ρ2 = Revoked.
+    rtc std_rel_pub ρ1 ρ2 → ρ2 = Temporary ∨ ρ2 = Revoked.
   Proof.
     intros Hρ1 Hrtc.
     inversion Hrtc; subst; auto.
-    apply std_rel_pub_Revoked in H as [-> | ->];auto.
-    - left. eapply std_rel_pub_rtc_Permanent;eauto.
-    - right. left. eapply std_rel_pub_rtc_Temporary;eauto.
+    apply std_rel_pub_Revoked in H as ->;auto.
+    left. eapply std_rel_pub_rtc_Temporary;eauto.
   Qed.
 
   (* ------------------------- DEFINITION STD STS CLASS -------------------------- *)
